Fix dgk extraction, add argmax c++ template

code/experimental/he/argmax/argmax.c
@@ -1,0 +1,23 @@
+#include "Hacl_Impl_Bignum_Misc.h"
+#include "Hacl_Impl_Bignum_Modular.h"
+#include "Hacl_Impl_HE_Paillier.h"
+#include "Hacl_Impl_Bignum_Comparison.h"
+#include "Hacl_Impl_HE_GM.h"
+
+#include <iostream>
+#include <random>
+
+
+void test_paillier () {
+    uint64_t a[1U] = { (uint64_t)128U };
+    uint64_t b[1U] = { (uint64_t)55U };
+    uint64_t* c = { 0, 0 };
+    std::cout << res0[0] << std::endl;
+}
+
+int main()
+{
+    test_paillier();
+    std::cout << "Benchmarks should be here" << std::endl;
+    return 0;
+}
